stuff

Rpn/Expr.lean
@@ -5,6 +5,13 @@ inductive BinaryOp where
   | div
 deriving BEq, Repr
 
+instance : ToString BinaryOp where
+  toString 
+    | .add => "+"
+    | .sub => "-"
+    | .mul => "*"
+    | .div => "/"
+
 inductive Expr where
   | int : Int -> Expr
   | binary : Expr -> BinaryOp -> Expr -> Expr
@@ -14,14 +21,65 @@ deriving BEq, Repr
 instance : Inhabited Expr where
   default := .error
 
-def Expr.eval (e : Expr) : Except String Int := do
+private def String.replicate (length : Nat) (char : Char) : String := 
+  (List.replicate length char).asString
+
+private def Expr.toStringPretty' (e : Expr) (depth : Nat) : String :=
+  let padding := String.replicate (depth * 2) ' '
   match e with
-  | .int i => .ok i
-  | .binary lhs .add rhs => .ok ((<-eval lhs) + (<-eval rhs))
-  | .binary lhs .sub rhs => .ok ((<-eval lhs) - (<-eval rhs))
-  | .binary lhs .mul rhs => .ok ((<-eval lhs) * (<-eval rhs))
-  | .binary lhs .div rhs => .ok ((<-eval lhs) / (<-eval rhs))
-  | .error => .error "encountered error node"
+  | .error => s!"{padding}<error>"
+  | .int i => s!"{padding}Int: {i}"
+  | .binary lhs op rhs => 
+      s!"{padding}Op :{op}\n{padding}{lhs.toStringPretty' (depth + 1)}\n{padding}{rhs.toStringPretty' (depth + 1)}"
 
 
+def Expr.toStringPretty (e : Expr) : String := e.toStringPretty' 0
+
+def Expr.eval? (e : Expr) : Option Int := do
+  match e with
+  | .int i => i
+  | .error => .none
+  | .binary lhs .add rhs => (<-eval? lhs) + (<-eval? rhs)
+  | .binary lhs .sub rhs => (<-eval? lhs) - (<-eval? rhs)
+  | .binary lhs .mul rhs => (<-eval? lhs) * (<-eval? rhs)
+  | .binary lhs .div rhs => (<-eval? lhs) / (<-eval? rhs)
+
+def Expr.isValid : Expr -> Bool 
+  | .error              => false
+  | .int _              => true
+  | .binary lhs _op rhs => lhs.isValid && rhs.isValid
+
+def Expr.children : Expr -> List Expr 
+  | .error            => []
+  | .int _            => []
+  | .binary lhs _ rhs => [lhs, rhs] ++ lhs.children ++ rhs.children
+
+def Expr.isError : Expr -> Bool
+  | .error => true
+  | _      => false
+
+
+theorem Expr.isValid_deep 
+  (lhs rhs : Expr) 
+  (op : BinaryOp) 
+  : (Expr.binary lhs op rhs).isValid -> (lhs.isValid ∧ rhs.isValid) := by 
+    intro is_valid
+    exact Bool.and_eq_true_iff.mp is_valid
+
+def Expr.eval (e : Expr) (is_valid : e.isValid) : Int := 
+  match e with
+  | .int i => i
+  | .binary lhs op rhs => 
+    let ⟨ lhs_valid, rhs_valid ⟩ := Expr.isValid_deep lhs rhs op is_valid
+
+    let lhs := eval lhs lhs_valid
+    let rhs := eval rhs rhs_valid
+
+    match op with
+    | .add => lhs + rhs
+    | .sub => lhs - rhs
+    | .mul => lhs * rhs
+    | .div => lhs / rhs
+
+    
 
