Main.lean
@@ -1,14 +1,14 @@
 import Rpn.Parser
 
-def processLine (line : String) : Except String Int :=
-  (parse line).eval
+def processLine (line : String) : Option Int :=
+  (parse line).eval?
 
 partial def repl (stream : IO.FS.Stream) : IO Unit := do
   let line <- stream.getLine
 
   match processLine line with
-  | .ok int => IO.println int
-  | .error msg => IO.eprintln msg
+  | .some int => IO.println int
+  | .none => IO.eprintln "error"
 
   repl stream
 
