Rpn/Util.lean
@@ -7,5 +7,45 @@ def List.headMatching { α : Type u } (as : List α) (p : α -> Bool) : List { a
     if proof : p a 
     then ⟨ a, proof ⟩ :: (as.headMatching p)
     else []
-        
 
+structure Span where
+  source         : String
+  start          : source.ValidPos
+  end'           : source.ValidPos
+  start_lt_end   : start < end'
+deriving BEq
+
+structure Spanned (α : Type u) where
+  val  : α
+  span : Span
+deriving BEq
+
+instance : Repr Span where
+  reprPrec span _prec := .text s!"{span.start.offset.byteIdx}..{span.end'.offset.byteIdx}"
+
+def Span.new (source : String) (startByte : Nat) (endByte : Nat) : Option Span := do
+  let start <- source.pos? ⟨ startByte ⟩ 
+  let end'  <- source.pos? ⟨ endByte ⟩ 
+
+  if start_lt_end : start < end' 
+  then .some ⟨ source, start, end', start_lt_end ⟩ 
+  else .none
+
+
+private theorem pos_lt_imp_le (s : String) (a b : s.ValidPos) : a < b -> a <= b := by
+  intro a_lt_b
+  refine String.ValidPos.le_iff.mpr ?_
+  have a_lt_b_offset : a.offset < b.offset := a_lt_b
+  exact String.Pos.Raw.le_of_lt a_lt_b
+
+
+def Span.text (span : Span) : String.Slice :=
+  ⟨ 
+    span.source,
+    span.start,
+    span.end',
+    (pos_lt_imp_le span.source span.start span.end') span.start_lt_end
+  ⟩ 
+
+def Span.lengthBytes (span : Span) : Nat := span.text.utf8ByteSize
+def Span.chars (span : Span) : List Char := span.text.chars.toList
